marshalling

ModularEngine/src/LogicEngine.FStar/marshall.fst
@@ -5,6 +5,10 @@ open Types
 logic function Strcat : list string -> string
 logic function ReprVar : var -> string
 logic function ReprVars : vars -> string
+logic function ReprConst: constant -> string
+logic function ReprSubstrateQueryTerm: ISubstrateQueryTerm -> string
+logic function ReprSubstrateUpdateTerm: ISubstrateUpdateTerm -> string
+logic function ReprFunc: func -> string
 logic function ReprMono : term -> string
 logic function ReprPoly : polyterm -> string
 assume forall (xs:vars) (t:term). 
@@ -35,8 +39,134 @@ assume forall (t:term). (ReprPoly (MonoTerm t)) = (ReprMono t)
          If we can do this totality proof in some other way, for example, 
          by providing an explicit ranking function, then we will have proved 
          that at least ReprPoly is at least a function. *)
+
+val printSubstrateConstant: object -> string
+val printSubstrateQuery: ISubstrateQueryTerm -> string
+val printSubstrateUpdate: ISubstrateUpdateTerm -> string
+
+val printList: ('a -> string) -> list 'a -> string -> string
+let rec printList printOne l delimiter =
+  match l with
+   | [] -> ""
+   | hd::tl -> 
+     (match tl with
+        | [] -> printOne hd
+        | _ -> strcat (printOne hd)
+               (strcat delimiter
+                (printList printOne tl delimiter)))
+
+val printOption: ('a -> string) -> option 'a -> string
+let printOption printA opt =
+  match opt with
+    | None -> "None"
+    | Some a -> strcat "Some("
+                (strcat (printA a)
+                 ")")
+
+val printTyp: typ -> string
+let printTyp ty = match ty with
+  | Infon -> "Infon"
+  | Principal -> "Principal"
+  | SubstrateUpdate -> "SubstrateUpdate"
+  | SubstrateQuery -> "SubstrateQuery"
+  | Action -> "Action"
+  | Condition -> "Condition"
+  | RuleT -> "RuleT"
+  | Evidence -> "Evidence"
+  | Boolean -> "Boolean"
+  | Int32 -> "Int32"
+  | Double -> "Double"
+  | String -> "String"
+
+val printVar: var -> string
+let printVar v = strcat "Var"
+                 (strcat (v.name)
+                 (strcat ", "
+                 (strcat (printTyp v.typ)
+                  ")")))
+
+val printPrincipal: principal -> string
+let printPrincipal p = p
+
+val printConst: constant -> string
+let printConst c = match c with
+  | TrueT -> "TrueT"
+  | FalseT -> "FalseT"
+  | SubstrateConstant o -> strcat "SubstrateConstant("
+                           (strcat (printSubstrateConstant o) ")")
+  | PrincipalConstant p ->
+    strcat "PrincipalConstant(" (strcat (printPrincipal p) ")")
+
+val printRelationInfon:relationInfon -> string
+val printFunc: func -> string
+val printMono: term -> string
+
+let printRelationInfon r =
+  strcat "RelationInfon("
+  (strcat (r.name)
+  (strcat ", "
+  (strcat (printTyp r.retType)
+  (strcat ", ["
+  (strcat (printList printTyp r.argsType "; ")
+  (strcat "], "
+  (printOption printMono r.identity)))))))
+ 
+let printFunc f = match f with
+  | SeqRule -> "SeqRule"
+  | EmptyRule -> "EmptyRule"
+  | Rule -> "Rule"
+  | RuleOnce -> "RuleOnce"
+  | SeqCondition -> "SeqCondition"
+  | EmptyCondition -> "EmptyCondition"
+  | WireCondition -> "WireCondition"
+  | KnownCondition -> "KnownCondition"
+  | SeqAction -> "SeqAction"
+  | EmptyAction -> "EmptyAction"
+  | Send -> "Send"
+  | JustifiedSend -> "JustifiedSend"
+  | JustifiedSay -> "JustifiedSay"
+  | Learn -> "Learn"
+  | Forget -> "Forget"
+  | Install -> "Install"
+  | Uninstall -> "Uninstall"
+  | Apply -> "Apply"
+  | Drop -> "Drop"
+  | EmptyInfon -> "EmptyInfon"
+  | AsInfon -> "AsInfon"
+  | AndInfon -> "AndInfon"
+  | ImpliesInfon -> "ImpliesInfon"
+  | SaidInfon -> "SaidInfon"
+  | JustifiedInfon -> "JustifiedInfon"
+  | EmptyEvidence -> "EmptyEvidence"
+  | SignatureEvidence -> "SignatureEvidence"
+  | ModusPonensEvidence -> "ModusPonensEvidence"
+  | AndEvidence -> "AndEvidence"
+  | AsInfonEvidence -> "AsInfonEvidence"
+  | RelationInfon r -> strcat "RelationInfon(" 
+                       (strcat (printRelationInfon r) ")")
+
+(*let printMono t = match t with
+  | Var x -> printVar x
+  | Const c -> printConst c
+  | SubstrateQueryTerm q -> printSubstrateQuery q
+  | SubstrateUpdateTerm u -> printSubstrateUpdate u
+  | App f ts -> strcat "(App "
+                (strcat (printFunc f)
+                (strcat " ["
+                (strcat (printList printMono ts "; ")
+                 "])"))) *)
+
 val printInfon: p:polyterm -> b:string{(ReprPoly p)=b}
-let printInfon p = raise "TODO"
+let printInfon p = 
+let str = match p with
+  | MonoTerm t -> printMono t
+  | ForallT xs t -> strcat "(Forall (" 
+                    (strcat (printList printVar xs ",")
+                    (strcat ") "
+                    (strcat (printMono t)
+                     ")"))) in
+assume ((ReprPoly p) = str);
+str
 
 (* Note: As for the printer, this function is recursive and so not in P. *)
 val parseInfon: b:string -> option (p:polyterm{(Net.Received b => Net.Received p) &&
